\section{Потенциалы электромагнитного поля. Лоренцевская калибровка.}

\begin{gather*}
    \mathrm{div}\vec{B}=0\Rightarrow \vec{B}=\mathrm{rot}\vec{A} \\
    \mathrm{rot}\vec{E}=-\frac{1}{c}\frac{\partial \vec{B}}{\partial t}=-\frac{1}{c}\frac{\partial  }{\partial t}\mathrm{rot}\vec{A}=-\frac{1}{c}\mathrm{rot}\frac{\partial \vec{A}}{\partial t}=\Rightarrow \mathrm{rot}\left( \vec{E}+\frac{1}{c}\frac{\partial \vec{A}}{\partial t}   \right)=0\Rightarrow \\
    \text{Итог:}    
\end{gather*}

\[
\boxed{\begin{aligned}
    \vec{B}&=\mathrm{rot}\vec{A} \\
    \vec{E}&=-\mathrm{grad}\varphi-\frac{1}{c}\frac{\partial \vec{A}}{\partial t}    
\end{aligned}}
\]

Калибровка:

\[
\begin{array}{l|l}
    \text{Если }\vec{A'}=\vec{A}+\grad f & \vec{B'}=\mathrm{rot}\vec{A'}=\mathrm{rot}\vec{A'}+\cancelto{0}{\mathrm{rot}(\grad f) }=\vec{B}  \\
    \vec{\varphi'}=\vec{\varphi}-\frac{1}{c}\frac{\partial f}{\partial t} & \vec{E'}=-\grad\varphi +\frac{1}{c}\grad \frac{\partial f}{\partial t}-\frac{1}{c} \frac{\partial \vec{A}}{\partial t}-\frac{1}{c} \frac{\partial}{\partial t} \grad f =\vec{E}   \\      
\end{array}
\]

\[
\begin{aligned}
\begin{cases}
    \mathrm{div}\vec{E}=4\pi\rho \\
    \mathrm{rot}\vec{E}=-\frac{1}{c} \frac{\partial \vec{H}}{\partial t} \\
    \mathrm{div}\vec{B}=0 \\
    \mathrm{rot}\vec{H}=\frac{4\pi}{c}\vec{j}+\frac{1}{c} \frac{\partial \vec{E}}{\partial t}    
\end{cases}
\text{ выполн.  }
\begin{cases}
    \vec{E}=-\grad \varphi -\frac{1}{c} \frac{\partial \vec{A}}{\partial t} \\
    \vec{H}=\mathrm{rot}\vec{A} 
\end{cases}
\end{aligned}
\]

\[
\begin{cases}
    -\Delta\varphi-\frac{1}{c}\frac{\partial}{\partial t}\grad \vec{A}=4\pi\rho \\
    \mathrm{grad div }\vec{A}-\Delta \vec{A} =\frac{4\pi}{c}\vec{j}+\frac{1}{c}  \frac{\partial }{\partial t} \left( \grad\varphi -\frac{1}{c} \frac{\partial \vec{A}}{\partial t}  \right)   
\end{cases}
\]

Если положить \( \mathrm{div}\vec{A}+\frac{1}{c} \frac{\partial\varphi}{/partial t}=0    \) \textit{-Лоренцевская калибровка}, получим:

\begin{gather*}
    \Delta\varphi-\frac{1}{c^2} \frac{\partial^2\varphi}{\partial t^2} =-4\pi\rho \\
    \Delta\vec{A}-\frac{1}{c^2} \frac{\partial^2}{\partial t^2}\vec{A}=-\frac{4\pi}{c}\vec{j}    
\end{gather*}

\[
\Delta:= \frac{\partial^2}{\partial x^2}+\frac{\partial^2}{\partial y^2} +\frac{\partial^2}{\partial z^2} ;\qquad \square :=\frac{\partial^2}{\partial x^2}+\frac{\partial^2}{\partial y^2} +\frac{\partial^2}{\partial z^2}-\frac{1}{c^2} \frac{\partial^2}{\partial t^2}
\]